more lemmas on subst

examples/hoare_logic/blocking_semantics/blocking_semantics_WP_progress_1.v
@@ -30,14 +30,15 @@ Inductive operator  :=
   | Omult : operator 
   | Ole : operator .
 
-(* Why3 assumption *)
-Definition ident  := Z.
+Parameter ident : Type.
+
+Parameter result: ident.
 
 (* Why3 assumption *)
 Inductive term  :=
   | Tvalue : value -> term 
-  | Tvar : Z -> term 
-  | Tderef : Z -> term 
+  | Tvar : ident -> term 
+  | Tderef : ident -> term 
   | Tbin : term -> operator -> term -> term .
 
 (* Why3 assumption *)
@@ -46,8 +47,8 @@ Inductive fmla  :=
   | Fand : fmla -> fmla -> fmla 
   | Fnot : fmla -> fmla 
   | Fimplies : fmla -> fmla -> fmla 
-  | Flet : Z -> term -> fmla -> fmla 
-  | Fforall : Z -> datatype -> fmla -> fmla .
+  | Flet : ident -> term -> fmla -> fmla 
+  | Fforall : ident -> datatype -> fmla -> fmla .
 
 Parameter map : forall (a:Type) (b:Type), Type.
 
@@ -74,7 +75,7 @@ Axiom Const : forall (a:Type) (b:Type), forall (b1:b) (a1:a),
   ((get (const b1:(map a b)) a1) = b1).
 
 (* Why3 assumption *)
-Definition env  := (map Z value).
+Definition env  := (map ident value).
 
 (* Why3 assumption *)
 Inductive list (a:Type) :=
@@ -86,21 +87,21 @@ Unset Contextual Implicit.
 Implicit Arguments Cons.
 
 (* Why3 assumption *)
-Definition stack  := (list (Z* value)%type).
+Definition stack  := (list (ident* value)%type).
 
-Parameter get_stack: Z -> (list (Z* value)%type) -> value.
+Parameter get_stack: ident -> (list (ident* value)%type) -> value.
 
-Axiom get_stack_def : forall (i:Z) (pi:(list (Z* value)%type)),
+Axiom get_stack_def : forall (i:ident) (pi:(list (ident* value)%type)),
   match pi with
   | Nil => ((get_stack i pi) = Vvoid)
   | (Cons (x, v) r) => ((x = i) -> ((get_stack i pi) = v)) /\ ((~ (x = i)) ->
       ((get_stack i pi) = (get_stack i r)))
   end.
 
-Axiom get_stack_eq : forall (x:Z) (v:value) (r:(list (Z* value)%type)),
-  ((get_stack x (Cons (x, v) r)) = v).
+Axiom get_stack_eq : forall (x:ident) (v:value) (r:(list (ident*
+  value)%type)), ((get_stack x (Cons (x, v) r)) = v).
 
-Axiom get_stack_neq : forall (x:Z) (i:Z) (v:value) (r:(list (Z*
+Axiom get_stack_neq : forall (x:ident) (i:ident) (v:value) (r:(list (ident*
   value)%type)), (~ (x = i)) -> ((get_stack i (Cons (x, v) r)) = (get_stack i
   r)).
 
@@ -121,7 +122,7 @@ Axiom eval_bin_def : forall (x:value) (op:operator) (y:value), match (x,
 
 (* Why3 assumption *)
 Set Implicit Arguments.
-Fixpoint eval_term(sigma:(map Z value)) (pi:(list (Z* value)%type))
+Fixpoint eval_term(sigma:(map ident value)) (pi:(list (ident* value)%type))
   (t:term) {struct t}: value :=
   match t with
   | (Tvalue v) => v
@@ -134,7 +135,7 @@ Unset Implicit Arguments.
 
 (* Why3 assumption *)
 Set Implicit Arguments.
-Fixpoint eval_fmla(sigma:(map Z value)) (pi:(list (Z* value)%type))
+Fixpoint eval_fmla(sigma:(map ident value)) (pi:(list (ident* value)%type))
   (f:fmla) {struct f}: Prop :=
   match f with
   | (Fterm t) => ((eval_term sigma pi t) = (Vbool true))
@@ -151,9 +152,9 @@ Fixpoint eval_fmla(sigma:(map Z value)) (pi:(list (Z* value)%type))
   end.
 Unset Implicit Arguments.
 
-Parameter subst_term: term -> Z -> Z -> term.
+Parameter subst_term: term -> ident -> ident -> term.
 
-Axiom subst_term_def : forall (e:term) (r:Z) (v:Z),
+Axiom subst_term_def : forall (e:term) (r:ident) (v:ident),
   match e with
   | ((Tvalue _)|(Tvar _)) => ((subst_term e r v) = e)
   | (Tderef x) => ((r = x) -> ((subst_term e r v) = (Tvar v))) /\
@@ -164,7 +165,7 @@ Axiom subst_term_def : forall (e:term) (r:Z) (v:Z),
 
 (* Why3 assumption *)
 Set Implicit Arguments.
-Fixpoint fresh_in_term(id:Z) (t:term) {struct t}: Prop :=
+Fixpoint fresh_in_term(id:ident) (t:term) {struct t}: Prop :=
   match t with
   | (Tvalue _) => True
   | (Tvar v) => ~ (id = v)
@@ -173,18 +174,18 @@ Fixpoint fresh_in_term(id:Z) (t:term) {struct t}: Prop :=
   end.
 Unset Implicit Arguments.
 
-Axiom eval_subst_term : forall (sigma:(map Z value)) (pi:(list (Z*
-  value)%type)) (e:term) (x:Z) (v:Z), (fresh_in_term v e) ->
+Axiom eval_subst_term : forall (sigma:(map ident value)) (pi:(list (ident*
+  value)%type)) (e:term) (x:ident) (v:ident), (fresh_in_term v e) ->
   ((eval_term sigma pi (subst_term e x v)) = (eval_term (set sigma x
   (get_stack v pi)) pi e)).
 
-Axiom eval_term_change_free : forall (t:term) (sigma:(map Z value)) (pi:(list
-  (Z* value)%type)) (id:Z) (v:value), (fresh_in_term id t) ->
-  ((eval_term sigma (Cons (id, v) pi) t) = (eval_term sigma pi t)).
+Axiom eval_term_change_free : forall (t:term) (sigma:(map ident value))
+  (pi:(list (ident* value)%type)) (id:ident) (v:value), (fresh_in_term id
+  t) -> ((eval_term sigma (Cons (id, v) pi) t) = (eval_term sigma pi t)).
 
 (* Why3 assumption *)
 Set Implicit Arguments.
-Fixpoint fresh_in_fmla(id:Z) (f:fmla) {struct f}: Prop :=
+Fixpoint fresh_in_fmla(id:ident) (f:fmla) {struct f}: Prop :=
   match f with
   | (Fterm e) => (fresh_in_term id e)
   | ((Fand f1 f2)|(Fimplies f1 f2)) => (fresh_in_fmla id f1) /\
@@ -198,7 +199,7 @@ Unset Implicit Arguments.
 
 (* Why3 assumption *)
 Set Implicit Arguments.
-Fixpoint subst(f:fmla) (x:Z) (v:Z) {struct f}: fmla :=
+Fixpoint subst(f:fmla) (x:ident) (v:ident) {struct f}: fmla :=
   match f with
   | (Fterm e) => (Fterm (subst_term e x v))
   | (Fand f1 f2) => (Fand (subst f1 x v) (subst f2 x v))
@@ -209,35 +210,52 @@ Fixpoint subst(f:fmla) (x:Z) (v:Z) {struct f}: fmla :=
   end.
 Unset Implicit Arguments.
 
-Axiom eval_subst : forall (f:fmla) (sigma:(map Z value)) (pi:(list (Z*
-  value)%type)) (x:Z) (v:Z), (fresh_in_fmla v f) -> ((eval_fmla sigma pi
-  (subst f x v)) <-> (eval_fmla (set sigma x (get_stack v pi)) pi f)).
+Axiom subst_fresh : forall (f:fmla) (x:ident) (v:ident), (fresh_in_fmla x
+  f) -> ((subst f x v) = f).
 
-Axiom eval_swap : forall (f:fmla) (sigma:(map Z value)) (pi:(list (Z*
-  value)%type)) (id1:Z) (id2:Z) (v1:value) (v2:value), (~ (id1 = id2)) ->
-  ((eval_fmla sigma (Cons (id1, v1) (Cons (id2, v2) pi)) f) <->
-  (eval_fmla sigma (Cons (id2, v2) (Cons (id1, v1) pi)) f)).
+Axiom let_subst : forall (t:term) (f:fmla) (x:ident) (id:ident) (idqt:ident),
+  ((subst (Flet x t f) id idqt) = (Flet x (subst_term t id idqt) (subst f id
+  idqt))).
 
-Axiom eval_change_free : forall (f:fmla) (sigma:(map Z value)) (pi:(list (Z*
-  value)%type)) (id:Z) (v:value), (fresh_in_fmla id f) -> ((eval_fmla sigma
-  (Cons (id, v) pi) f) <-> (eval_fmla sigma pi f)).
+Axiom eval_subst : forall (f:fmla) (sigma:(map ident value)) (pi:(list
+  (ident* value)%type)) (x:ident) (v:ident), (fresh_in_fmla v f) ->
+  ((eval_fmla sigma pi (subst f x v)) <-> (eval_fmla (set sigma x
+  (get_stack v pi)) pi f)).
+
+Axiom eval_swap : forall (f:fmla) (sigma:(map ident value)) (pi:(list (ident*
+  value)%type)) (id1:ident) (id2:ident) (v1:value) (v2:value),
+  (~ (id1 = id2)) -> ((eval_fmla sigma (Cons (id1, v1) (Cons (id2, v2) pi))
+  f) <-> (eval_fmla sigma (Cons (id2, v2) (Cons (id1, v1) pi)) f)).
+
+Axiom eval_change_free : forall (f:fmla) (sigma:(map ident value)) (pi:(list
+  (ident* value)%type)) (id:ident) (v:value), (fresh_in_fmla id f) ->
+  ((eval_fmla sigma (Cons (id, v) pi) f) <-> (eval_fmla sigma pi f)).
+
+(* Why3 assumption *)
+Definition valid_fmla(p:fmla): Prop := forall (sigma:(map ident value))
+  (pi:(list (ident* value)%type)), (eval_fmla sigma pi p).
+
+Axiom let_equiv : forall (id:ident) (idqt:ident) (t:term) (f:fmla),
+  forall (sigma:(map ident value)) (pi:(list (ident* value)%type)),
+  (eval_fmla sigma pi (Flet idqt t (subst f id idqt))) -> (eval_fmla sigma pi
+  (Flet id t f)).
 
 (* Why3 assumption *)
 Inductive expr  :=
   | Evalue : value -> expr 
   | Ebin : expr -> operator -> expr -> expr 
-  | Evar : Z -> expr 
-  | Ederef : Z -> expr 
-  | Eassign : Z -> expr -> expr 
+  | Evar : ident -> expr 
+  | Ederef : ident -> expr 
+  | Eassign : ident -> expr -> expr 
   | Eseq : expr -> expr -> expr 
-  | Elet : Z -> expr -> expr -> expr 
+  | Elet : ident -> expr -> expr -> expr 
   | Eif : expr -> expr -> expr -> expr 
   | Eassert : fmla -> expr 
   | Ewhile : expr -> fmla -> expr -> expr .
 
 (* Why3 assumption *)
 Set Implicit Arguments.
-Fixpoint fresh_in_expr(id:Z) (e:expr) {struct e}: Prop :=
+Fixpoint fresh_in_expr(id:ident) (e:expr) {struct e}: Prop :=
   match e with
   | (Evalue _) => True
   | ((Eseq e1 e2)|(Ebin e1 _ e2)) => (fresh_in_expr id e1) /\
@@ -256,123 +274,127 @@ Fixpoint fresh_in_expr(id:Z) (e:expr) {struct e}: Prop :=
 Unset Implicit Arguments.
 
 (* Why3 assumption *)
-Inductive one_step : (map Z value) -> (list (Z* value)%type) -> expr -> (map
-  Z value) -> (list (Z* value)%type) -> expr -> Prop :=
-  | one_step_var : forall (sigma:(map Z value)) (pi:(list (Z* value)%type))
-      (v:Z), (one_step sigma pi (Evar v) sigma pi (Evalue (get_stack v pi)))
-  | one_step_deref : forall (sigma:(map Z value)) (pi:(list (Z* value)%type))
-      (v:Z), (one_step sigma pi (Ederef v) sigma pi (Evalue (get sigma v)))
-  | one_step_bin_ctxt1 : forall (sigma:(map Z value)) (sigmaqt:(map Z value))
-      (pi:(list (Z* value)%type)) (piqt:(list (Z* value)%type)) (op:operator)
-      (e1:expr) (e1qt:expr) (e2:expr), (one_step sigma pi e1 sigmaqt piqt
-      e1qt) -> (one_step sigma pi (Ebin e1 op e2) sigmaqt piqt (Ebin e1qt op
-      e2))
-  | one_step_bin_ctxt2 : forall (sigma:(map Z value)) (sigmaqt:(map Z value))
-      (pi:(list (Z* value)%type)) (piqt:(list (Z* value)%type)) (op:operator)
-      (v1:value) (e2:expr) (e2qt:expr), (one_step sigma pi e2 sigmaqt piqt
-      e2qt) -> (one_step sigma pi (Ebin (Evalue v1) op e2) sigmaqt piqt
-      (Ebin (Evalue v1) op e2qt))
-  | one_step_bin_value : forall (sigma:(map Z value)) (sigmaqt:(map Z value))
-      (pi:(list (Z* value)%type)) (piqt:(list (Z* value)%type)) (op:operator)
-      (v1:value) (v2:value), (one_step sigma pi (Ebin (Evalue v1) op
-      (Evalue v2)) sigmaqt piqt (Evalue (eval_bin v1 op v2)))
-  | one_step_assign_ctxt : forall (sigma:(map Z value)) (sigmaqt:(map Z
-      value)) (pi:(list (Z* value)%type)) (piqt:(list (Z* value)%type)) (x:Z)
-      (e:expr) (eqt:expr), (one_step sigma pi e sigmaqt piqt eqt) ->
-      (one_step sigma pi (Eassign x e) sigmaqt piqt (Eassign x eqt))
-  | one_step_assign_value : forall (sigma:(map Z value)) (pi:(list (Z*
-      value)%type)) (x:Z) (v:value), (one_step sigma pi (Eassign x
-      (Evalue v)) (set sigma x v) pi (Evalue Vvoid))
-  | one_step_seq_ctxt : forall (sigma:(map Z value)) (sigmaqt:(map Z value))
-      (pi:(list (Z* value)%type)) (piqt:(list (Z* value)%type)) (e1:expr)
-      (e1qt:expr) (e2:expr), (one_step sigma pi e1 sigmaqt piqt e1qt) ->
-      (one_step sigma pi (Eseq e1 e2) sigmaqt piqt (Eseq e1qt e2))
-  | one_step_seq_value : forall (sigma:(map Z value)) (pi:(list (Z*
+Inductive one_step : (map ident value) -> (list (ident* value)%type) -> expr
+  -> (map ident value) -> (list (ident* value)%type) -> expr -> Prop :=
+  | one_step_var : forall (sigma:(map ident value)) (pi:(list (ident*
+      value)%type)) (v:ident), (one_step sigma pi (Evar v) sigma pi
+      (Evalue (get_stack v pi)))
+  | one_step_deref : forall (sigma:(map ident value)) (pi:(list (ident*
+      value)%type)) (v:ident), (one_step sigma pi (Ederef v) sigma pi
+      (Evalue (get sigma v)))
+  | one_step_bin_ctxt1 : forall (sigma:(map ident value)) (sigmaqt:(map ident
+      value)) (pi:(list (ident* value)%type)) (piqt:(list (ident*
+      value)%type)) (op:operator) (e1:expr) (e1qt:expr) (e2:expr),
+      (one_step sigma pi e1 sigmaqt piqt e1qt) -> (one_step sigma pi (Ebin e1
+      op e2) sigmaqt piqt (Ebin e1qt op e2))
+  | one_step_bin_ctxt2 : forall (sigma:(map ident value)) (sigmaqt:(map ident
+      value)) (pi:(list (ident* value)%type)) (piqt:(list (ident*
+      value)%type)) (op:operator) (v1:value) (e2:expr) (e2qt:expr),
+      (one_step sigma pi e2 sigmaqt piqt e2qt) -> (one_step sigma pi
+      (Ebin (Evalue v1) op e2) sigmaqt piqt (Ebin (Evalue v1) op e2qt))
+  | one_step_bin_value : forall (sigma:(map ident value)) (sigmaqt:(map ident
+      value)) (pi:(list (ident* value)%type)) (piqt:(list (ident*
+      value)%type)) (op:operator) (v1:value) (v2:value), (one_step sigma pi
+      (Ebin (Evalue v1) op (Evalue v2)) sigmaqt piqt (Evalue (eval_bin v1 op
+      v2)))
+  | one_step_assign_ctxt : forall (sigma:(map ident value)) (sigmaqt:(map
+      ident value)) (pi:(list (ident* value)%type)) (piqt:(list (ident*
+      value)%type)) (x:ident) (e:expr) (eqt:expr), (one_step sigma pi e
+      sigmaqt piqt eqt) -> (one_step sigma pi (Eassign x e) sigmaqt piqt
+      (Eassign x eqt))
+  | one_step_assign_value : forall (sigma:(map ident value)) (pi:(list
+      (ident* value)%type)) (x:ident) (v:value), (one_step sigma pi
+      (Eassign x (Evalue v)) (set sigma x v) pi (Evalue Vvoid))
+  | one_step_seq_ctxt : forall (sigma:(map ident value)) (sigmaqt:(map ident
+      value)) (pi:(list (ident* value)%type)) (piqt:(list (ident*
+      value)%type)) (e1:expr) (e1qt:expr) (e2:expr), (one_step sigma pi e1
+      sigmaqt piqt e1qt) -> (one_step sigma pi (Eseq e1 e2) sigmaqt piqt
+      (Eseq e1qt e2))
+  | one_step_seq_value : forall (sigma:(map ident value)) (pi:(list (ident*
       value)%type)) (e:expr), (one_step sigma pi (Eseq (Evalue Vvoid) e)
       sigma pi e)
-  | one_step_let_ctxt : forall (sigma:(map Z value)) (sigmaqt:(map Z value))
-      (pi:(list (Z* value)%type)) (piqt:(list (Z* value)%type)) (id:Z)
-      (e1:expr) (e1qt:expr) (e2:expr), (one_step sigma pi e1 sigmaqt piqt
-      e1qt) -> (one_step sigma pi (Elet id e1 e2) sigmaqt piqt (Elet id e1qt
-      e2))
-  | one_step_let_value : forall (sigma:(map Z value)) (pi:(list (Z*
-      value)%type)) (id:Z) (v:value) (e:expr), (one_step sigma pi (Elet id
-      (Evalue v) e) sigma (Cons (id, v) pi) e)
-  | one_step_if_ctxt : forall (sigma:(map Z value)) (sigmaqt:(map Z value))
-      (pi:(list (Z* value)%type)) (piqt:(list (Z* value)%type)) (e1:expr)
-      (e1qt:expr) (e2:expr) (e3:expr), (one_step sigma pi e1 sigmaqt piqt
-      e1qt) -> (one_step sigma pi (Eif e1 e2 e3) sigmaqt piqt (Eif e1qt e2
-      e3))
-  | one_step_if_true : forall (sigma:(map Z value)) (pi:(list (Z*
+  | one_step_let_ctxt : forall (sigma:(map ident value)) (sigmaqt:(map ident
+      value)) (pi:(list (ident* value)%type)) (piqt:(list (ident*
+      value)%type)) (id:ident) (e1:expr) (e1qt:expr) (e2:expr),
+      (one_step sigma pi e1 sigmaqt piqt e1qt) -> (one_step sigma pi (Elet id
+      e1 e2) sigmaqt piqt (Elet id e1qt e2))
+  | one_step_let_value : forall (sigma:(map ident value)) (pi:(list (ident*
+      value)%type)) (id:ident) (v:value) (e:expr), (one_step sigma pi
+      (Elet id (Evalue v) e) sigma (Cons (id, v) pi) e)
+  | one_step_if_ctxt : forall (sigma:(map ident value)) (sigmaqt:(map ident
+      value)) (pi:(list (ident* value)%type)) (piqt:(list (ident*
+      value)%type)) (e1:expr) (e1qt:expr) (e2:expr) (e3:expr),
+      (one_step sigma pi e1 sigmaqt piqt e1qt) -> (one_step sigma pi (Eif e1
+      e2 e3) sigmaqt piqt (Eif e1qt e2 e3))
+  | one_step_if_true : forall (sigma:(map ident value)) (pi:(list (ident*
       value)%type)) (e1:expr) (e2:expr), (one_step sigma pi
       (Eif (Evalue (Vbool true)) e1 e2) sigma pi e1)
-  | one_step_if_false : forall (sigma:(map Z value)) (pi:(list (Z*
+  | one_step_if_false : forall (sigma:(map ident value)) (pi:(list (ident*
       value)%type)) (e1:expr) (e2:expr), (one_step sigma pi
       (Eif (Evalue (Vbool false)) e1 e2) sigma pi e2)
-  | one_step_assert : forall (sigma:(map Z value)) (pi:(list (Z*
+  | one_step_assert : forall (sigma:(map ident value)) (pi:(list (ident*
       value)%type)) (f:fmla), (eval_fmla sigma pi f) -> (one_step sigma pi
       (Eassert f) sigma pi (Evalue Vvoid))
-  | one_step_while : forall (sigma:(map Z value)) (pi:(list (Z* value)%type))
-      (cond:expr) (inv:fmla) (body:expr), (eval_fmla sigma pi inv) ->
-      (one_step sigma pi (Ewhile cond inv body) sigma pi (Eif cond (Eseq body
-      (Ewhile cond inv body)) (Evalue Vvoid))).
+  | one_step_while : forall (sigma:(map ident value)) (pi:(list (ident*
+      value)%type)) (cond:expr) (inv:fmla) (body:expr), (eval_fmla sigma pi
+      inv) -> (one_step sigma pi (Ewhile cond inv body) sigma pi (Eif cond
+      (Eseq body (Ewhile cond inv body)) (Evalue Vvoid))).
 
 (* Why3 assumption *)
-Inductive many_steps : (map Z value) -> (list (Z* value)%type) -> expr
-  -> (map Z value) -> (list (Z* value)%type) -> expr -> Z -> Prop :=
-  | many_steps_refl : forall (sigma:(map Z value)) (pi:(list (Z*
+Inductive many_steps : (map ident value) -> (list (ident* value)%type)
+  -> expr -> (map ident value) -> (list (ident* value)%type) -> expr
+  -> Z -> Prop :=
+  | many_steps_refl : forall (sigma:(map ident value)) (pi:(list (ident*
       value)%type)) (e:expr), (many_steps sigma pi e sigma pi e 0%Z)
-  | many_steps_trans : forall (sigma1:(map Z value)) (sigma2:(map Z value))
-      (sigma3:(map Z value)) (pi1:(list (Z* value)%type)) (pi2:(list (Z*
-      value)%type)) (pi3:(list (Z* value)%type)) (e1:expr) (e2:expr)
-      (e3:expr) (n:Z), (one_step sigma1 pi1 e1 sigma2 pi2 e2) ->
-      ((many_steps sigma2 pi2 e2 sigma3 pi3 e3 n) -> (many_steps sigma1 pi1
-      e1 sigma3 pi3 e3 (n + 1%Z)%Z)).
+  | many_steps_trans : forall (sigma1:(map ident value)) (sigma2:(map ident
+      value)) (sigma3:(map ident value)) (pi1:(list (ident* value)%type))
+      (pi2:(list (ident* value)%type)) (pi3:(list (ident* value)%type))
+      (e1:expr) (e2:expr) (e3:expr) (n:Z), (one_step sigma1 pi1 e1 sigma2 pi2
+      e2) -> ((many_steps sigma2 pi2 e2 sigma3 pi3 e3 n) ->
+      (many_steps sigma1 pi1 e1 sigma3 pi3 e3 (n + 1%Z)%Z)).
 
-Axiom steps_non_neg : forall (sigma1:(map Z value)) (sigma2:(map Z value))
-  (pi1:(list (Z* value)%type)) (pi2:(list (Z* value)%type)) (e1:expr)
-  (e2:expr) (n:Z), (many_steps sigma1 pi1 e1 sigma2 pi2 e2 n) ->
+Axiom steps_non_neg : forall (sigma1:(map ident value)) (sigma2:(map ident
+  value)) (pi1:(list (ident* value)%type)) (pi2:(list (ident* value)%type))
+  (e1:expr) (e2:expr) (n:Z), (many_steps sigma1 pi1 e1 sigma2 pi2 e2 n) ->
   (0%Z <= n)%Z.
 
-Axiom many_steps_seq : forall (sigma1:(map Z value)) (sigma3:(map Z value))
-  (pi1:(list (Z* value)%type)) (pi3:(list (Z* value)%type)) (e1:expr)
-  (e2:expr) (n:Z), (many_steps sigma1 pi1 (Eseq e1 e2) sigma3 pi3
-  (Evalue Vvoid) n) -> exists sigma2:(map Z value), exists pi2:(list (Z*
-  value)%type), exists n1:Z, exists n2:Z, (many_steps sigma1 pi1 e1 sigma2
-  pi2 (Evalue Vvoid) n1) /\ ((many_steps sigma2 pi2 e2 sigma3 pi3
+Axiom many_steps_seq : forall (sigma1:(map ident value)) (sigma3:(map ident
+  value)) (pi1:(list (ident* value)%type)) (pi3:(list (ident* value)%type))
+  (e1:expr) (e2:expr) (n:Z), (many_steps sigma1 pi1 (Eseq e1 e2) sigma3 pi3
+  (Evalue Vvoid) n) -> exists sigma2:(map ident value), exists pi2:(list
+  (ident* value)%type), exists n1:Z, exists n2:Z, (many_steps sigma1 pi1 e1
+  sigma2 pi2 (Evalue Vvoid) n1) /\ ((many_steps sigma2 pi2 e2 sigma3 pi3
   (Evalue Vvoid) n2) /\ (n = ((1%Z + n1)%Z + n2)%Z)).
 
-Axiom many_steps_let : forall (sigma1:(map Z value)) (sigma3:(map Z value))
-  (pi1:(list (Z* value)%type)) (pi3:(list (Z* value)%type)) (id:Z) (e1:expr)
-  (e2:expr) (v2:value) (n:Z), (many_steps sigma1 pi1 (Elet id e1 e2) sigma3
-  pi3 (Evalue v2) n) -> exists sigma2:(map Z value), exists pi2:(list (Z*
-  value)%type), exists v1:value, exists n1:Z, exists n2:Z, (many_steps sigma1
-  pi1 e1 sigma2 pi2 (Evalue v1) n1) /\ ((many_steps sigma2 (Cons (id, v1)
-  pi2) e2 sigma3 pi3 (Evalue v2) n2) /\ (n = ((1%Z + n1)%Z + n2)%Z)).
+Axiom many_steps_let : forall (sigma1:(map ident value)) (sigma3:(map ident
+  value)) (pi1:(list (ident* value)%type)) (pi3:(list (ident* value)%type))
+  (id:ident) (e1:expr) (e2:expr) (v2:value) (n:Z), (many_steps sigma1 pi1
+  (Elet id e1 e2) sigma3 pi3 (Evalue v2) n) -> exists sigma2:(map ident
+  value), exists pi2:(list (ident* value)%type), exists v1:value,
+  exists n1:Z, exists n2:Z, (many_steps sigma1 pi1 e1 sigma2 pi2 (Evalue v1)
+  n1) /\ ((many_steps sigma2 (Cons (id, v1) pi2) e2 sigma3 pi3 (Evalue v2)
+  n2) /\ (n = ((1%Z + n1)%Z + n2)%Z)).
 
-Axiom one_step_change_free : forall (e:expr) (eqt:expr) (sigma:(map Z value))
-  (sigmaqt:(map Z value)) (pi:(list (Z* value)%type)) (piqt:(list (Z*
-  value)%type)) (id:Z) (v:value), (fresh_in_expr id e) -> ((one_step sigma
-  (Cons (id, v) pi) e sigmaqt piqt eqt) -> (one_step sigma pi e sigmaqt piqt
-  eqt)).
-
-(* Why3 assumption *)
-Definition valid_fmla(p:fmla): Prop := forall (sigma:(map Z value)) (pi:(list
-  (Z* value)%type)), (eval_fmla sigma pi p).
+Axiom one_step_change_free : forall (e:expr) (eqt:expr) (sigma:(map ident
+  value)) (sigmaqt:(map ident value)) (pi:(list (ident* value)%type))
+  (piqt:(list (ident* value)%type)) (id:ident) (v:value), (fresh_in_expr id
+  e) -> ((one_step sigma (Cons (id, v) pi) e sigmaqt piqt eqt) ->
+  (one_step sigma pi e sigmaqt piqt eqt)).
 
 (* Why3 assumption *)
 Definition valid_triple(p:fmla) (e:expr) (q:fmla): Prop := forall (sigma:(map
-  Z value)) (pi:(list (Z* value)%type)), (eval_fmla sigma pi p) ->
-  forall (sigmaqt:(map Z value)) (piqt:(list (Z* value)%type)) (v:value)
-  (n:Z), (many_steps sigma pi e sigmaqt piqt (Evalue v) n) ->
-  (eval_fmla sigmaqt (Cons ((-1%Z)%Z, v) piqt) q).
+  ident value)) (pi:(list (ident* value)%type)), (eval_fmla sigma pi p) ->
+  forall (sigmaqt:(map ident value)) (piqt:(list (ident* value)%type))
+  (v:value) (n:Z), (many_steps sigma pi e sigmaqt piqt (Evalue v) n) ->
+  (eval_fmla sigmaqt (Cons (result, v) piqt) q).
 
 (* Why3 assumption *)
 Definition total_valid_triple(p:fmla) (e:expr) (q:fmla): Prop :=
-  forall (sigma:(map Z value)) (pi:(list (Z* value)%type)), (eval_fmla sigma
-  pi p) -> exists sigmaqt:(map Z value), exists piqt:(list (Z* value)%type),
-  exists v:value, exists n:Z, (many_steps sigma pi e sigmaqt piqt (Evalue v)
-  n) /\ (eval_fmla sigmaqt (Cons ((-1%Z)%Z, v) piqt) q).
+  forall (sigma:(map ident value)) (pi:(list (ident* value)%type)),
+  (eval_fmla sigma pi p) -> exists sigmaqt:(map ident value),
+  exists piqt:(list (ident* value)%type), exists v:value, exists n:Z,
+  (many_steps sigma pi e sigmaqt piqt (Evalue v) n) /\ (eval_fmla sigmaqt
+  (Cons (result, v) piqt) q).
 
 Parameter set1 : forall (a:Type), Type.
 
@@ -456,28 +478,28 @@ Unset Contextual Implicit.
 Axiom all_def : forall (a:Type), forall (x:a), (mem x (all :(set1 a))).
 
 (* Why3 assumption *)
-Definition assigns(sigma:(map Z value)) (a:(set1 Z)) (sigmaqt:(map Z
-  value)): Prop := forall (i:Z), (~ (mem i a)) -> ((get sigma
+Definition assigns(sigma:(map ident value)) (a:(set1 ident)) (sigmaqt:(map
+  ident value)): Prop := forall (i:ident), (~ (mem i a)) -> ((get sigma
   i) = (get sigmaqt i)).
 
-Axiom assigns_refl : forall (sigma:(map Z value)) (a:(set1 Z)),
+Axiom assigns_refl : forall (sigma:(map ident value)) (a:(set1 ident)),
   (assigns sigma a sigma).
 
-Axiom assigns_trans : forall (sigma1:(map Z value)) (sigma2:(map Z value))
-  (sigma3:(map Z value)) (a:(set1 Z)), ((assigns sigma1 a sigma2) /\
-  (assigns sigma2 a sigma3)) -> (assigns sigma1 a sigma3).
+Axiom assigns_trans : forall (sigma1:(map ident value)) (sigma2:(map ident
+  value)) (sigma3:(map ident value)) (a:(set1 ident)), ((assigns sigma1 a
+  sigma2) /\ (assigns sigma2 a sigma3)) -> (assigns sigma1 a sigma3).
 
-Axiom assigns_union_left : forall (sigma:(map Z value)) (sigmaqt:(map Z
-  value)) (s1:(set1 Z)) (s2:(set1 Z)), (assigns sigma s1 sigmaqt) ->
-  (assigns sigma (union s1 s2) sigmaqt).
+Axiom assigns_union_left : forall (sigma:(map ident value)) (sigmaqt:(map
+  ident value)) (s1:(set1 ident)) (s2:(set1 ident)), (assigns sigma s1
+  sigmaqt) -> (assigns sigma (union s1 s2) sigmaqt).
 
-Axiom assigns_union_right : forall (sigma:(map Z value)) (sigmaqt:(map Z
-  value)) (s1:(set1 Z)) (s2:(set1 Z)), (assigns sigma s2 sigmaqt) ->
-  (assigns sigma (union s1 s2) sigmaqt).
+Axiom assigns_union_right : forall (sigma:(map ident value)) (sigmaqt:(map
+  ident value)) (s1:(set1 ident)) (s2:(set1 ident)), (assigns sigma s2
+  sigmaqt) -> (assigns sigma (union s1 s2) sigmaqt).
 
 (* Why3 assumption *)
 Set Implicit Arguments.
-Fixpoint expr_writes(e:expr) (w:(set1 Z)) {struct e}: Prop :=
+Fixpoint expr_writes(e:expr) (w:(set1 ident)) {struct e}: Prop :=
   match e with
   | ((Evalue _)|((Evar _)|((Ederef _)|(Eassert _)))) => True
   | (Ebin e1 _ e2) => (expr_writes e1 w) /\ (expr_writes e2 w)
@@ -490,7 +512,7 @@ Fixpoint expr_writes(e:expr) (w:(set1 Z)) {struct e}: Prop :=
   end.
 Unset Implicit Arguments.
 
-Parameter fresh_from: fmla -> expr -> Z.
+Parameter fresh_from: fmla -> expr -> ident.
 
 Axiom fresh_from_fmla : forall (e:expr) (f:fmla),
   (fresh_in_fmla (fresh_from f e) f).
@@ -504,35 +526,45 @@ Parameter abstract_effects: expr -> fmla -> fmla.
 Set Implicit Arguments.
 Fixpoint wp(e:expr) (q:fmla) {struct e}: fmla :=
   match e with
-  | (Evalue v) => (Flet (-1%Z)%Z (Tvalue v) q)
-  | (Evar v) => (Flet (-1%Z)%Z (Tvar v) q)
-  | (Ederef x) => (Flet (-1%Z)%Z (Tderef x) q)
+  | (Evalue v) => (Flet result (Tvalue v) q)
+  | (Evar v) => (Flet result (Tvar v) q)
+  | (Ederef x) => (Flet result (Tderef x) q)
   | (Eassert f) => (Fand f (Fimplies f q))
   | (Eseq e1 e2) => (wp e1 (wp e2 q))
-  | (Elet id e1 e2) => (wp e1 (Flet id (Tvar (-1%Z)%Z) (wp e2 q)))
+  | (Elet id e1 e2) => (wp e1 (Flet id (Tvar result) (wp e2 q)))
   | (Ebin e1 op e2) => let t1 := (fresh_from q e) in let t2 :=
-      (fresh_from (Fand (Fterm (Tvar t1)) q) e) in let qqt := (Flet (-1%Z)%Z
+      (fresh_from (Fand (Fterm (Tvar t1)) q) e) in let qqt := (Flet result
       (Tbin (Tvar t1) op (Tvar t2)) q) in let f := (wp e2 (Flet t2
-      (Tvar (-1%Z)%Z) qqt)) in (wp e1 (Flet t1 (Tvar (-1%Z)%Z) f))
-  | (Eassign x e1) => let id := (fresh_from q e1) in let qqt :=
-      (Flet (-1%Z)%Z (Tvalue Vvoid) q) in (wp e1 (Flet id (Tvar (-1%Z)%Z)
-      (subst qqt x id)))
-  | (Eif e1 e2 e3) => let f := (Fand (Fimplies (Fterm (Tvar (-1%Z)%Z)) (wp e2
-      q)) (Fimplies (Fnot (Fterm (Tvar (-1%Z)%Z))) (wp e3 q))) in (wp e1 f)
+      (Tvar result) qqt)) in (wp e1 (Flet t1 (Tvar result) f))
+  | (Eassign x e1) => let id := (fresh_from q e1) in let qqt := (Flet result
+      (Tvalue Vvoid) q) in (wp e1 (Flet id (Tvar result) (subst qqt x id)))
+  | (Eif e1 e2 e3) => let f := (Fand (Fimplies (Fterm (Tvar result)) (wp e2
+      q)) (Fimplies (Fnot (Fterm (Tvar result))) (wp e3 q))) in (wp e1 f)
   | (Ewhile cond inv body) => (Fand inv (abstract_effects body (wp cond
-      (Fand (Fimplies (Fand (Fterm (Tvar (-1%Z)%Z)) inv) (wp body inv))
-      (Fimplies (Fand (Fnot (Fterm (Tvar (-1%Z)%Z))) inv) q)))))
+      (Fand (Fimplies (Fand (Fterm (Tvar result)) inv) (wp body inv))
+      (Fimplies (Fand (Fnot (Fterm (Tvar result))) inv) q)))))
   end.
 Unset Implicit Arguments.
 
-Axiom wp_conj : forall (sigma:(map Z value)) (pi:(list (Z* value)%type))
-  (e:expr) (p:fmla) (q:fmla), (eval_fmla sigma pi (wp e (Fand p q))) <->
-  ((eval_fmla sigma pi (wp e p)) /\ (eval_fmla sigma pi (wp e q))).
+Axiom wp_subst : forall (e:expr) (q:fmla) (id:ident) (idqt:ident),
+  (fresh_in_expr id e) -> ((subst (wp e q) id idqt) = (wp e (subst q id
+  idqt))).
 
-Axiom wp_reduction : forall (sigma:(map Z value)) (sigmaqt:(map Z value))
-  (pi:(list (Z* value)%type)) (piqt:(list (Z* value)%type)) (e:expr)
-  (eqt:expr) (q:fmla), ((one_step sigma pi e sigmaqt piqt eqt) /\
-  (eval_fmla sigma pi (wp e q))) -> (eval_fmla sigmaqt piqt (wp eqt q)).
+Axiom wp_implies : forall (p:fmla) (q:fmla), (forall (sigma:(map ident
+  value)) (pi:(list (ident* value)%type)), (eval_fmla sigma pi p) ->
+  (eval_fmla sigma pi q)) -> forall (sigma:(map ident value)) (pi:(list
+  (ident* value)%type)) (e:expr), (eval_fmla sigma pi (wp e p)) ->
+  (eval_fmla sigma pi (wp e q)).
+
+Axiom wp_conj : forall (sigma:(map ident value)) (pi:(list (ident*
+  value)%type)) (e:expr) (p:fmla) (q:fmla), (eval_fmla sigma pi (wp e (Fand p
+  q))) <-> ((eval_fmla sigma pi (wp e p)) /\ (eval_fmla sigma pi (wp e q))).
+
+Axiom wp_reduction : forall (sigma:(map ident value)) (sigmaqt:(map ident
+  value)) (pi:(list (ident* value)%type)) (piqt:(list (ident* value)%type))
+  (e:expr) (eqt:expr), (one_step sigma pi e sigmaqt piqt eqt) ->
+  forall (q:fmla), (eval_fmla sigma pi (wp e q)) -> (eval_fmla sigmaqt piqt
+  (wp eqt q)).
 
 (* Why3 assumption *)
 Definition not_a_value(e:expr): Prop :=
@@ -545,10 +577,11 @@ Axiom decide_value : forall (e:expr), (not_a_value e) \/ exists v:value,
   (e = (Evalue v)).
 
 (* Why3 goal *)
-Theorem progress : forall (e:expr) (sigma:(map Z value)) (pi:(list (Z*
-  value)%type)) (q:fmla), ((eval_fmla sigma pi (wp e q)) /\
-  (not_a_value e)) -> exists sigmaqt:(map Z value), exists piqt:(list (Z*
-  value)%type), exists eqt:expr, (one_step sigma pi e sigmaqt piqt eqt).
+Theorem progress : forall (e:expr) (sigma:(map ident value)) (pi:(list
+  (ident* value)%type)) (q:fmla), ((eval_fmla sigma pi (wp e q)) /\
+  (not_a_value e)) -> exists sigmaqt:(map ident value), exists piqt:(list
+  (ident* value)%type), exists eqt:expr, (one_step sigma pi e sigmaqt piqt
+  eqt).
 induction e.
 simpl; tauto.
 (* case 1: e = bin e1 op e2 *)
@@ -614,7 +647,7 @@ generalize (IHe _ _ _ (conj h1 H)).
 intros (sigma' & pi' & e' & h).
 exists sigma'.
 exists pi'.
-exists (Eassign z e').
+exists (Eassign i e').
 apply one_step_assign_ctxt; auto.
 (* case 4.2: e' is a value *)
 elim H; clear H; intros v He_v.
